start renaming

formalization/typing.v
@@ -28,29 +28,29 @@ Fixpoint lfl_Allₛ {A} {P : A -> Type} {Pₚ : forall a, P a -> Type} (HPₚ : 
 Check lfl_Allₛ.
 
 Parameter term : Type.
-Parameter tCase : term -> list term -> term.
+Parameter switch : term -> list term -> term.
 
 Inductive typing : term -> term -> Type :=
-| typing_tCase (discr ind : term) (branches : list term) (return_type : term) :
+| typing_switch (discr ind : term) (branches : list term) (return_type : term) :
           typing discr ind -> All (fun a => typing a return_type) branches ->
-          typing (tCase discr branches) return_type.
+          typing (switch discr branches) return_type.
 
 Fixpoint typing_elim (P : forall t T, typing t T -> Type)
-  (PtCase : forall discr ind branches return_type,
+  (Pswitch : forall discr ind branches return_type,
             forall (ty_discr : typing discr ind), P discr ind ty_discr ->
             forall (ty_br : All (fun a => typing a return_type) branches),
               Allₛ (fun a ty_a => P a return_type ty_a) ty_br ->
-            P _ _ (typing_tCase discr ind branches return_type ty_discr ty_br)) :
+            P _ _ (typing_switch discr ind branches return_type ty_discr ty_br)) :
     forall t T ty_tT, P t T ty_tT :=
   fun t T ty_tT => match ty_tT with
-  | typing_tCase discr ind br return_type ty_discr ty_br =>
-      PtCase discr ind br return_type ty_discr (typing_elim P PtCase _ _ ty_discr)
-        ty_br (lfl_Allₛ (fun t => typing_elim P PtCase t return_type) _ ty_br)
+  | typing_switch discr ind br return_type ty_discr ty_br =>
+      Pswitch discr ind br return_type ty_discr (typing_elim P Pswitch _ _ ty_discr)
+        ty_br (lfl_Allₛ (fun t => typing_elim P Pswitch t return_type) _ ty_br)
   end.
 
 Inductive typing_mut : term -> term -> Type :=
-| typing_mut_tCase (discr ind : term) (branches : list term) (return_type : term) :
-    typing_mut discr ind -> All_mut return_type branches -> typing_mut (tCase discr branches) return_type
+| typing_mut_switch (discr ind : term) (branches : list term) (return_type : term) :
+    typing_mut discr ind -> All_mut return_type branches -> typing_mut (switch discr branches) return_type
 with All_mut : term -> list term -> Type :=
 | All_mut_nil return_type : All_mut return_type []
 | All_mut_cons return_type a l : typing_mut a return_type -> All_mut return_type l -> All_mut return_type (a::l).
@@ -92,16 +92,16 @@ Scheme typing_mut_All_mut_rec := Induction for typing_mut Sort Type
 Definition typing_mut_All_mut_rec2
     (P : forall t t0 : term, typing_mut t t0 -> Type)
     (P0 : forall (t : term) (l : list term), All_mut t l -> Type)
-    (Ptyping_mut_tCase : forall discr ind branches return_type,
+    (Ptyping_mut_switch : forall discr ind branches return_type,
       forall ty_discr : typing_mut discr ind, P _ _ ty_discr ->
       forall ty_br : All_mut return_type branches, P0 _ _ ty_br ->
-      P _ _  (typing_mut_tCase discr ind branches return_type ty_discr ty_br))
+      P _ _  (typing_mut_switch discr ind branches return_type ty_discr ty_br))
     (P0All_mut_nil  : forall return_type, P0 _ _ (All_mut_nil return_type))
     (P0All_mut_cons : forall return_type a l, forall ty_a, P _ _ ty_a ->
       forall ty_l, P0 _ _ ty_l -> P0 _ _ (All_mut_cons return_type a l ty_a ty_l)) :
   forall t T ty_tT, P t T ty_tT.
 Proof.
-  apply (typing_mut_All_mut_rec P P0 Ptyping_mut_tCase P0All_mut_nil P0All_mut_cons).
+  apply (typing_mut_All_mut_rec P P0 Ptyping_mut_switch P0All_mut_nil P0All_mut_cons).
 Qed.
 
 (* just relabling *)
@@ -152,19 +152,19 @@ Proof.
     assumption.
 Qed.
 
-Definition typing_tCase' discr ind branches return_type :
+Definition typing_switch' discr ind branches return_type :
     typing_mut discr ind -> All (fun a => typing_mut a return_type) branches ->
-    typing_mut (tCase discr branches) return_type :=
+    typing_mut (switch discr branches) return_type :=
   fun ty_discr ty_br =>
-  typing_mut_tCase discr ind branches return_type ty_discr (All_to_All_mut ty_br).
+  typing_mut_switch discr ind branches return_type ty_discr (All_to_All_mut ty_br).
 
 Definition typing_elim2
   (P : forall t T, typing_mut t T -> Type)
-  (PtCase' : forall discr ind branches return_type,
+  (Pswitch' : forall discr ind branches return_type,
             forall (ty_discr : typing_mut discr ind), P discr ind ty_discr ->
             forall (ty_br : All (fun a => typing_mut a return_type) branches),
               Allₛ (fun a ty_a => P a return_type ty_a) ty_br ->
-            P _ _ (typing_tCase' discr ind branches return_type ty_discr ty_br)) :
+            P _ _ (typing_switch' discr ind branches return_type ty_discr ty_br)) :
     forall t T ty_tT, P t T ty_tT.
 Proof.
   unshelve eapply typing_mut_All_mut_rec with
@@ -173,19 +173,19 @@ Proof.
            Allₛ (fun a ty_a => P a return_type ty_a) (All_mut_to_All ty_br)).
   - intros discr ind branches return_type ty_discr Pty_discr ty_br Pty_br.
     rewrite (All_mut_eq ty_br).
-    apply ((PtCase' discr ind branches return_type ty_discr Pty_discr (All_mut_to_All ty_br) Pty_br)).
+    apply ((Pswitch' discr ind branches return_type ty_discr Pty_discr (All_mut_to_All ty_br) Pty_br)).
     (* wont type check as P can't be inferred *)
     (* fun discr ind branches return_type ty_discr Pty_discr ty_br Pty_br =>
-      (All_mut_eq ty_br) # (PtCase' discr ind branches return_type ty_discr Pty_discr (All_mut_to_All ty_br) Pty_br). *)
+      (All_mut_eq ty_br) # (Pswitch' discr ind branches return_type ty_discr Pty_discr (All_mut_to_All ty_br) Pty_br). *)
   - exact (fun return_type => Allₛ_nil).
   - exact (fun return_type a l ty_a Pty_a ty_l Pty_l => Allₛ_cons a l ty_a Pty_a ((All_mut_to_All ty_l)) Pty_l).
 Defined.
 
-Definition typing_elim2_tCase' :
-  forall P PtCase' discr ind branches return_type ty_discr ty_br,
-    typing_elim2 P PtCase' _ _ (typing_tCase' _ _ _ _ ty_discr ty_br)
-  = PtCase' _ _ _ _ ty_discr (typing_elim2 P PtCase' discr ind ty_discr) ty_br
-      (lfl_Allₛ (fun t => typing_elim2 P PtCase' t return_type) branches ty_br).
+Definition typing_elim2_switch' :
+  forall P Pswitch' discr ind branches return_type ty_discr ty_br,
+    typing_elim2 P Pswitch' _ _ (typing_switch' _ _ _ _ ty_discr ty_br)
+  = Pswitch' _ _ _ _ ty_discr (typing_elim2 P Pswitch' discr ind ty_discr) ty_br
+      (lfl_Allₛ (fun t => typing_elim2 P Pswitch' t return_type) branches ty_br).
 Proof.
   (* It does NOT compute *)
   Fail reflexivity.
